Extending relation classes with more properties

dafny/set-theory/binRelOnS.dfy
@@ -4,16 +4,24 @@ module binRelS
 {    
     import opened binRelST
     /*
-    Abstraction of a finite binary relation on a 
-    set, S. Underlying representation is a pair: 
-    the domain set, S, and a set of pairs over S.
+    Abstraction of a polymorphic finite binary 
+    relation over a set, S, of elements of type,
+    T. 
+    
+    The concrete representatation of a value of
+    this type is just an object of the binRelOnST
+    class, where both of its type parameters are
+    T, and where the domain and codomain sets are
+    just S. This class specializes (restricts) 
+    the more general binRelOnST class. Most of 
+    the operations of this class just "delegate"
+    to the underlying relation object. 
     */ 
     class binRelOnS<T(!new,==)>
     {
         /*
-        We represent a binary relation, R, over a set,
-        T, as a value of the type of binary relations
-        over two types, but where both types are just S.
+        Concrete representation: a binary relation
+        on T X T.
         */
         var r: binRelOnST<T,T>;
 
@@ -28,37 +36,103 @@ module binRelS
             r.Valid() && r.dom() == r.codom()
         }
 
-
         /*
-        Constructor just instantiates a binary relation
-        on S X T with the type, T, of the single set over
-        which the current relation is defined, setting the
-        domain and codomain sets to be the same set, elts.
+        This constructor instantiates a binary relation
+        on S X T using type, T, for both type parameters,
+        a single set for the both the domain and codomain
+        sets, and a set of T-T pairs as the relation, with
+        the constraint that values in the relation be from
+        the domain/codomain set.
         */
         constructor(elts: set<T>, pairs: set<(T,T)>)
+            /*
+            The relation has to be over the given set.
+            */
             requires forall x, y :: 
                 (x, y) in pairs ==> x in elts && y in elts;
-            ensures r.d == elts && 
-                    r.c == elts && r.r == pairs
+            
+            /*
+            Dafny can't see into *method* bodies, so 
+            explain as part of the spec what this method '
+            achieves. Dafny needs this information for 
+            later verifications.
+            */
+            ensures r.d == elts && r.c == elts && r.r == pairs
+
+            /*
+            The constructor leaves the object in a valid 
+            state. All other operations require that an 
+            object be Valid as a
+            */
             ensures Valid();
          {
             r := new binRelOnST(elts,elts,pairs);
         }
 
         /*
-        Return domain set
+        Accessor (projection) function: return the domain 
+        set.
         */
         function method dom(): set<T>
-            reads this;
-            reads r;
+
+            /*
+            Every operation (function, method) of this 
+            class except for the constructor require that
+            an object be in a valid state for the operation
+            to be applied. Every method is also required to
+            ensure that it leaves this object in a valid
+            state, so ensures Valid() is also included 
+            below and in every other method. The idea is
+            that the constructor establises the property
+            of being valid, and every method preserves it,
+            so it is an *invariant* property of objecst of
+            this type. Specifying and ensuring preservation
+            of state invariants of objects is essential,
+            and the failure to do so properly is a major
+            source of bugs in code.
+            */
             requires Valid();
+ 
+            /*
+            Dafny needs to know what values a function reads
+            in order to know what values its results might
+            depend on, for purposes of later verifications.
+            The "reads this" specification element informs
+            the verifier that this function might read any 
+            of the fields of this object.
+            */
+            reads this;
+
+            /*
+            This specification element, "reads r" tells Dafny
+            that his function can call functions that in turn
+            read fields of r.
+            */
+            reads r;
+
+            /*
+            As explained above, this (and every) operation is
+            requires to leave this object in a valid state.
+            */
             ensures Valid();
         {
+            /*
+            After all that, we just "delegate" this operation
+            to the corresponding operation of the underlying
+            binRelOnST object, by calling r.dom(). That this
+            operation leaves the object in a valid state thus
+            relies on r.dom() doing so. And that is the case,
+            because Dafny verifies that function as doing so.
+            */
             r.dom()
         }
 
         /*
-        Return codomain set
+        Accessor (projection) function: return the codomain 
+        set. The detailed explanations for the preceding 
+        function apply more or less directly to this and
+        other operations in this class. We do not repeat
+        the comments in every class.
         */
         function method codom(): set<T>
             reads this;
@@ -70,7 +144,8 @@ module binRelS
         }
 
         /*
-        Return set of ordered pairs
+        Accessor/projection function: return the 
+        relation (pair set).
         */
         function method rel(): set<(T,T)>
             reads this;
@@ -83,7 +158,8 @@ module binRelS
 
 
         /*
-        Return true iff the relation is single-valued (a function)
+        Return true if and only if the relation is 
+        single-valued (i.e., actually a function)
         */
         predicate method isFunction()
             reads this;
@@ -91,18 +167,35 @@ module binRelS
             requires Valid();
             ensures Valid();
         {
+            /* Again, we just "delegate" this.isFunction()
+            to r (the underlying binRelOnST object, by calling
+            r.isFunction().
+            */
             r.isFunction()  
         }
 
         
         /*
-        Return true iff the relation is a function and is injective
+        Return true iff this relation is a function, 
+        and it is an injective function, in particular.
+        
+        The properties of being injective, surjective, 
+        or bijective apply to single-valued relations,
+        i.e., to functions. We thus restrict the next
+        three operations to apply only when this object
+        satisfies is a function, which is to say that it
+        satisfies the isFunction() predicate. We thus
+        add this.isFunction() as a pre-condition to each
+        of these operations. (We leave off the "this.", 
+        as it's implicitly there already.) We then just
+        delegate legal calls to these operations to the
+        corresponding operations on r.
         */
         predicate method isInjective()
             reads this;
             reads r;
             requires Valid();
-            requires isFunction();
+            requires isFunction();  // newprecondition
             ensures Valid();
         {
             r.isInjective()
@@ -110,7 +203,8 @@ module binRelS
         
         
         /*
-        Return true iff the relation is a function and is surjective 
+        Return true iff the relation is a function and 
+        it is a surjective function, in particular. 
         */
         predicate method isSurjective()
             reads this;
@@ -123,7 +217,8 @@ module binRelS
         }
 
         /*
-        Return true iff the relation a function and is bijective
+        Return true iff the relation is a function 
+        and is bijective, in particular. 
         */
 
         predicate method isBijective()
@@ -138,7 +233,9 @@ module binRelS
 
 
        /*
-        Return true iff the relation is total (relative to its domain)
+        Return true iff the relation is total 
+        (i.e., defined on every element of its
+        domain set).
         */
         predicate method isTotal()
             reads this;
@@ -151,7 +248,8 @@ module binRelS
 
         
         /*
-        Return true iff the relation is partial (relative to its domain set)
+        Return true iff the relation is partial 
+        (not total relative to its domain set).
         */
         predicate method isPartial()
             reads this;
@@ -164,15 +262,28 @@ module binRelS
 
 
         /*
-        Return true iff the relation is reflexive
+        Return true iff this relation is reflexive.
+        To be reflexive a relation must map every
+        element of its domain to itself. 
+
+        This funciton provides a good simple example
+        of a unversally quantified predicate in Dafny.
+        It can be read as "forall x (implicitly of type
+        T), if x is in the domain of this relation then
+        (x,x) is in the relation." The following few
+        functions are written in the same style. What
+        you have in these cases, then, is simply the
+        mathematical definitions of these fundamental
+        properties of relations expressed using Dafny 
+        syntax.
         */
         predicate method isReflexive()
             reads this;
             reads r;
             requires Valid();
-            ensures Valid();        
+            ensures Valid(); 
         {
-            forall x :: x in dom() ==> (x, x) in rel() 
+            forall x :: x in dom() ==> (x, x) in rel()
         }
 
 
@@ -221,34 +332,177 @@ module binRelS
         }
 
 
+        predicate method isPreorder()
+                    reads this;
+            reads r;
+            requires Valid();
+            ensures Valid();
+        {
+            isReflexive() && isTransitive() 
+        }
+
+
+        predicate method isAntisymmetric()
+            reads this;
+            reads r;
+            requires Valid();
+            ensures Valid();
+
+        {
+            forall x, y ::     x in dom()   &&   y in dom() &&
+                           (x,y) in rel() && (y,x) in rel() ==> 
+                           x == y
+        }
+
+
+        predicate method isPartialOrder()
+            reads this;
+            reads r;
+            requires Valid();
+            ensures Valid();
+
+        {
+            isReflexive() && isTransitive() && isAntisymmetric()
+        }
+
         /*
-        Compute image of a domain element under this relation.
+        The image of a domain value under a relation
+        is the set of values to which the relation
+        maps that domain element. This method provides
+        this behavior. It computes and returns the 
+        image of a domain element under this relation.
+        It requires that the given value actually be
+        in the domain set. Note that if the relation
+        is not defined for an element in its domain,
+        the image of that value will simply be the
+        empty set.
         */
         function method image(k: T): (r: set<T>)
             reads this;
             reads r;
             requires Valid(); 
+            requires k in dom();
             ensures Valid();
         {
             r.image(k)
         }
 
 
+        /*
+        The image of a *set* of domain elements is just
+        the set of values that the relation maps those
+        elements to. It basically "looks up" each domain
+        element and returns the union of all the images
+        of those values. A precondition for calling this
+        function is that all argument values (in ks) be
+        in the domain of this relation.
+        */
+        function method imageOfSet(ks: set<T>): (r: set<T>)
+            reads this;
+            reads r;
+            requires Valid(); 
+            requires forall k :: k in ks ==> k in dom();  
+            ensures Valid();
+        {
+            r.imageOfSet(ks)
+        }
+
+
+        /*
+        Given an element in the range of a relation, its
+        preimage is the set of elements in in the domain
+        that map to it. This function returns the preimage
+        of a given value in the range of this relation. It
+        is a precondition that v be in the codomain of this
+        relation.
+        */
+        function method preimage(v: T): (r: set<T>)
+            reads this;
+            reads r;
+            requires Valid(); 
+            requires v in codom();
+            ensures Valid();
+        {
+            r.preimage(v)
+        }
+
 
         /*
         Compute image of a domain element under this relation.
         */
-        method imagef(k: T) returns (ret: T)
+        function method preimageOfSet(vs: set<T>): (r: set<T>)
+            reads this;
+            reads r;
             requires Valid(); 
-            requires isFunction();
-            requires isTotal();   // ensures defined for every value
-            requires k in dom();  // ensures function is non-empty
-            ensures ret in image(k);
-            ensures this == old(this);
-            ensures r == old(r);
+            requires forall v :: v in vs ==> v in codom();
             ensures Valid();
         {
-            ret := r.imagef(k);
+            r.preimageOfSet(vs)
         }
+
+
+        /*
+        A relation is said to be defined for a given
+        domain element, k, if the relation maps k to 
+        at least one value in the codomain. 
+        */
+        predicate method isDefinedFor(k: T)
+            reads this;
+            reads r;
+            requires Valid();
+            requires k in dom();
+            ensures Valid();
+        {
+            r.isDefinedFor(k)
+        }
+
+        /*
+        If this relation is a function, then we can
+        "apply" it to a single value, on which this
+        function is defined, to get a single result. 
+        */
+        method apply(k: T) returns (ret: T)
+            requires Valid(); 
+            requires k in dom();   // only ask about domain values
+            requires isFunction(); // only ask if this is a function
+            requires isTotal();   // that is defined for every value
+            requires isDefinedFor(k);  // and that is non-empty
+//            ensures ret in image(k);  // want |image(k)| == 1, too
+            ensures Valid();
+        {
+            ret := r.fimage(k);
+        }
+
+        method convertToBinRelOnST() returns (c: binRelOnST<T,T>)
+            requires Valid();
+            ensures c.Valid();
+            ensures c.dom() == dom() && 
+                    c.codom() == codom() && 
+                    c.rel() == rel();
+        {
+            c := new binRelOnST(dom(), codom(), rel());
+        }
+    }
+
+
+    method composeSS<T>(g: binRelOnS<T>, f: binRelOnS<T>) 
+        returns (h : binRelOnST<T,T>)
+        requires f.Valid();
+        requires g.Valid();
+        ensures h.Valid();
+        ensures h.dom() == f.dom();
+        ensures h.codom() == g.codom();
+        ensures h.rel() == set r, s, t | 
+                r in f.dom() &&
+                s in f.codom() &&
+                (r, s) in f.rel() &&
+                s in g.dom() && 
+                t in g.codom() &&
+                (s, t) in g.rel() ::
+                (r, t)
+    {
+        var f' := f.convertToBinRelOnST();
+        var g' := g.convertToBinRelOnST();
+        h := composeRST(g',f');
     }
 }
