dafny/set-theory/binRelOnST.dfy
@@ -222,7 +222,7 @@ module binRelST
         the given value. Be sure value is in domain
         before calling this function.
         */
-        predicate method definedAt(k: S)
+        predicate method isDefinedFor(k: S)
             requires Valid()
             requires k in d;
             reads this;
@@ -248,7 +248,7 @@ module binRelST
 
 
         /*
-        Compute image set of a value under this relation.
+        Compute image set of a single value under this relation.
         */
         function method image(k: S): (vals: set<T>)
             reads this;
@@ -259,19 +259,55 @@ module binRelST
         }
 
 
+/*
+        Compute image set of a set of values under this relation.
+        */
+        function method imageOfSet(ks: set<S>): (vals: set<T>)
+            reads this;
+            requires Valid(); 
+            ensures Valid();
+        {
+            set x, y | x in d && y in c && (x, y) in r && x in ks :: y
+        }
+
+        /*
+        Compute preimage set of an individual value under this relation.
+        */
+        function method preimage(v: S): (vals: set<T>)
+            reads this;
+            requires Valid(); 
+            ensures Valid();
+        {
+            set x, y | x in d && y in c && (x, y) in r && x == v :: y
+        }
+
+
+        /*
+        Compute preimage set of a set of values under this relation.
+        */
+        function method preimageOfSet(ks: set<S>): (vals: set<T>)
+            reads this;
+            requires Valid(); 
+            ensures Valid();
+        {
+            set x, y | x in d && y in c && (x, y) in r && x in ks :: y
+        }
+
+
+
         /*
         Compute image of a domain element under this relation.
         This code assumes there is exactly one element in the 
-        set from which the value is drawn, but this assumption
-        is not yet verified.
+        set from which the value is drawn (but this assumption
+        is not yet verified).
         */
-        method imagef(k: S) returns (val: T)
+        method fimage(k: S) returns (val: T)
             requires Valid(); 
             requires isFunction();  // ensures single-valuedness
             requires k in d;        // ensures function is non-empty
-            requires definedAt(k);
-            ensures this == old(this);
-            ensures d == old(d) && c == old(c) && r == old(r);
+            requires isDefinedFor(k);
+            //ensures this == old(this);
+            //ensures d == old(d) && c == old(c) && r == old(r);
             ensures Valid();
             /*
             Make behavior of this opaque *method* visible as a spec
@@ -282,7 +318,46 @@ module binRelST
             var s := set x, y | 
                         x in d && y in c && (x, y) in r && x == k :: y;
             val :| val in s;
-            // assert |s| == 1; -- believed true but doesn't verify
+            assert |s| >= 1; // believed true but doesn't verify
         }
+    }
+
+    
+    /*
+    The composition, h, of two functions, f and g, where f maps 
+    R-values to S-values, and g maps S-values to T-values, is
+    a relation that maps R-values to T-values, where h contains
+    a pair (s,r) if and only if there is some t such that (s,t)
+    is in f, and (t,r) is in g. The composition of relations is
+    a special case of the composition of functions. More details
+    to be discussed in class.
+    */
+    method composeRST<R,S,T>(g: binRelOnST<S,T>, f: binRelOnST<R,S>) 
+        returns (h : binRelOnST<R,T>)
+        requires f.Valid();
+        requires g.Valid();
+        ensures h.Valid();
+        ensures h.dom() == f.dom();
+        ensures h.codom() == g.codom();
+        ensures h.rel() == set r, s, t | 
+                r in f.dom() &&
+                s in f.codom() &&
+                (r, s) in f.rel() &&
+                s in g.dom() && 
+                t in g.codom() &&
+                (s, t) in g.rel() ::
+                (r, t)
+    {
+        h := new binRelOnST<R,T>(
+            f.dom(),  
+            g.codom(), 
+            set r, s, t | 
+                r in f.dom() &&
+                s in f.codom() &&
+                (r, s) in f.rel() &&
+                s in g.dom() && 
+                t in g.codom() &&
+                (s, t) in g.rel() ::
+                (r, t));
     }
 }
